More work in completeness proof.

SeparationLogic/Complete_Flat.v
@@ -4,6 +4,8 @@ Require Import Logic.lib.Bijection.
 Require Import Logic.lib.Countable.
 Require Import Logic.MinimunLogic.LogicBase.
 Require Import Logic.MinimunLogic.MinimunLogic.
+Require Import Logic.MinimunLogic.ContextProperty.
+Require Import Logic.MinimunLogic.HenkinCompleteness.
 Require Import Logic.PropositionalLogic.Syntax.
 Require Import Logic.SeparationLogic.Syntax.
 Require Import Logic.PropositionalLogic.KripkeSemantics.
@@ -47,6 +49,444 @@ Instance SM: Semantics L MD := FlatSemanticsModel.SM Var.
 Instance kiSM (M: Kmodel): KripkeIntuitionisticSemantics L MD M SM := FlatSemanticsModel.kiSM Var M.
 Instance fsSM (M: Kmodel): FlatSemantics.FlatSemantics L MD M SM := FlatSemanticsModel.fsSM Var M.
 Instance UsSM (M: Kmodel): UnitarySemantics L MD M SM := FlatSemanticsModel.UsSM Var M.
+Locate derivable_closed.
+Definition DCS (Gamma: ProofTheory L): Type := sig (fun Phi =>
+  derivable_closed Phi /\
+  orp_witnessed Phi /\
+  consistent Phi).
+
+Lemma DCS_ext {Gamma: ProofTheory L}: forall m n: DCS Gamma,
+  m = n <-> (forall x: expr, proj1_sig m x <-> proj1_sig n x).
+Proof.
+  intros.
+  split; [intros; subst; reflexivity |].
+  intros.
+  destruct m as [m ?H], n as [n ?H].
+  simpl in H.
+  assert (m = n).
+  + apply Extensionality_Ensembles.
+    split; unfold Included, Ensembles.In; intros; apply H; auto.
+  + subst n.
+    assert (H0 = H1) by apply proof_irrelevance.
+    subst H1; auto.
+Qed.
+
+Definition canonical_frame {Gamma: ProofTheory L}: FlatSemanticsModel.frame.
+  refine (FlatSemanticsModel.Build_frame (DCS Gamma) (fun a b => Included _ (proj1_sig b) (proj1_sig a)) _ (fun a b c => forall x y, proj1_sig a x -> proj1_sig b y -> proj1_sig c (x * y)) _ _ _).
+  Unshelve.
+  Focus 5. shelve.
+  Focus 5. shelve.
+  Focus 5. shelve.
+  Focus 4. {
+    constructor.
+    + hnf; intros.
+      hnf; intros; auto.
+    + hnf; intros.
+      hnf; intros; auto.
+  } Unfocus.
+  + constructor.
+    - intros; simpl in *.
+      intros x y ? ?.
+      specialize (H y x H1 H0).
+      pose proof proj2_sig m.
+      destruct H2 as [? _].
+      rewrite derivable_closed_element_derivable in H |- *. 2: auto.
+Focus 2. {
+exact H2.
+Defined.
+
+Program Definition canonical_eval: Var -> KripkeSemantics.sem canonical_frame :=
+  fun p a => a (PropositionalLanguage.varp p).
+Next Obligation.
+  apply H; auto.
+Qed.
+
+Definition canonical_Kmodel: KripkeSemantics.Kmodel Var :=
+  KripkeSemantics.Build_Kmodel Var canonical_frame canonical_eval.
+
+Definition canonical_model (Phi: DCS): model :=
+  KripkeSemantics.Build_model Var canonical_Kmodel Phi.
+
+Lemma Lindenbaum_lemma:
+  forall Phi x,
+    ~ Phi |-- x ->
+    exists Psi,
+      Included _ Phi Psi /\
+      ~ Psi |-- x /\
+      derivable_closed Psi /\
+      orp_witnessed Psi /\
+      consistent Psi.
+Proof.
+  intros.
+  assert (Countable expr) by (apply PropositionalLanguage.formula_countable; auto).
+  set (step :=
+          fun n Phi x0 =>
+             Phi x0 \/
+            (X x0 n /\
+             ~ (Union _ Phi (Singleton _ x0)) |-- x)).
+  exists (LindenbaumConstruction step Phi).
+  assert (Included expr Phi (LindenbaumConstruction step Phi) /\
+          ~ LindenbaumConstruction step Phi |-- x /\
+          (~ LindenbaumConstruction step Phi |-- x ->
+           derivable_closed (LindenbaumConstruction step Phi)) /\
+          (~ LindenbaumConstruction step Phi |-- x ->
+           orp_witnessed (LindenbaumConstruction step Phi))).
+  Focus 2. {
+    destruct H0 as [? [? [? ?]]].
+    split; [| split; [| split; [| split]]]; auto.
+    rewrite consistent_spec.
+    intro; apply H1.
+    pose proof deduction_falsep_elim _ x H4.
+    auto.
+  } Unfocus.
+  split; [| split; [| split]].
+  + apply (Lindenbaum_spec_included _ _ 0).
+  + apply (Lindenbaum_spec_pos _ _
+            (fun xs => |-- multi_imp xs x)
+            (fun Phi => Phi |-- x)).
+    - intros; apply derivable_provable.
+    - intros ? ? ? ?; left; auto.
+    - apply H.
+    - intros.
+      destruct (Classical_Prop.classic (exists x0, X x0 n /\ ~ (Union _ S (Singleton _ x0)) |-- x)) as [[x0 [? ?]] |].
+      * intro; apply H2; clear H2.
+        eapply deduction_weaken; [| exact H3].
+        hnf; intros ? [? | [? ?]]; [left; auto |].
+        pose proof in_inj _ _ X _ _ _ H1 H2.
+        subst; right; constructor.
+      * intro; apply H0; clear H0.
+        eapply deduction_weaken; [| exact H2].
+        hnf; intros ? [? | [? ?]]; [auto |].
+        exfalso; apply H1; clear H1.
+        exists x0; auto.
+  + intros; hnf; intros.
+    destruct (im_inj _ _ X x0) as [n ?].
+    apply (Lindenbaum_spec_neg _ _ _ (S n)).
+    simpl.
+    unfold step at 1.
+    right; split; auto.
+    intro.
+    rewrite deduction_theorem in H3.
+    eapply deduction_weaken in H3; [| apply (Lindenbaum_spec_included _ _ n)].
+    pose proof deduction_modus_ponens _ _ _ H1 H3.
+    auto.
+  + intros; hnf; intros x0 y0 ?.
+    destruct (im_inj _ _ X x0) as [nx ?].
+    destruct (im_inj _ _ X y0) as [ny ?].
+    assert (LindenbaumChain step Phi (S nx) x0 \/ LindenbaumChain step Phi (S ny) y0) as HH;
+      [| destruct HH as [HH | HH]; apply Lindenbaum_spec_neg in HH; auto].
+    simpl.
+    unfold step at 1 3.
+    assert (~ Union _ (LindenbaumChain step Phi nx) (Singleton _ x0) |-- x \/
+            ~ Union _ (LindenbaumChain step Phi ny) (Singleton _ y0) |-- x) as HH;
+      [| destruct HH as [HH | HH]; auto].
+    apply Classical_Prop.not_and_or; intros [? ?].
+    rewrite deduction_theorem in H4, H5.
+    eapply deduction_weaken in H4; [| apply (Lindenbaum_spec_included _ _ nx)].
+    eapply deduction_weaken in H5; [| apply (Lindenbaum_spec_included _ _ ny)].
+    pose proof deduction_orp_elim (LindenbaumConstruction step Phi) x0 y0 x H4 H5.
+    apply (derivable_assum _ (x0 || y0)) in H1.
+    pose proof deduction_modus_ponens _ _ _ H1 H6.
+    auto.
+Qed.
+
+Lemma truth_lemma: forall (Phi: DCS) x, canonical_model Phi |= x <-> proj1_sig Phi x.
+Proof.
+  intros.
+  pose proof (fun Phi: DCS => derivable_closed_element_derivable (proj1_sig Phi) (proj1 (proj2_sig Phi))).
+  revert Phi.
+  induction x; try solve [inversion H0]; intros.
+  + specialize (IHx1 Phi).
+    specialize (IHx2 Phi).
+    pose proof DCS_andp_iff (proj1_sig Phi) (proj1 (proj2_sig Phi)) x1 x2.
+    simpl in *.
+    unfold KripkeSemantics.sem_and.
+    tauto.
+  + specialize (IHx1 Phi).
+    specialize (IHx2 Phi).
+    pose proof DCS_orp_iff (proj1_sig Phi) (proj1 (proj2_sig Phi)) (proj1 (proj2 (proj2_sig Phi))) x1 x2.
+    simpl in *.
+    unfold KripkeSemantics.sem_or.
+    tauto.
+  + split.
+    - intros.
+      rewrite H.
+      apply (@deduction_theorem _ _ _ _ (IntuitionisticPropositionalLogic.mpG Var)).
+      apply Classical_Prop.NNPP; intro.
+      pose proof Lindenbaum_lemma _ _ H1.
+      destruct H2 as [Psi [? [? ?]]].
+      hnf in H0.
+      specialize (H0 (exist _ Psi H4)).
+      assert (Included _ (proj1_sig Phi) Psi) by (hnf; intros; apply H2; left; auto).
+      specialize (H0 H5).
+      simpl in IHx1, IHx2.
+      simpl in H0.
+      rewrite IHx1, IHx2 in H0; simpl in H0.
+      assert (Psi x1) by (apply H2; right; constructor).
+      specialize (H0 H6).
+      specialize (H (exist _ Psi H4) x2); simpl in H.
+      rewrite H in H0; auto.
+    - intros.
+      hnf; intros Psi ?H.
+      change DCS in Psi.
+      simpl in H1.
+      simpl in IHx1, IHx2.
+      rewrite IHx1, IHx2.
+      intros.
+      rewrite H in H0, H2 |- *.
+      eapply deduction_weaken in H0; [| exact H1].
+      eapply deduction_modus_ponens; [exact H2 | exact H0].
+  + simpl.
+    split; [intros [] | intros].
+    rewrite H in H0.
+    pose proof proj2_sig Phi.
+    destruct H1 as [_ [_ ?]].
+    rewrite consistent_spec in H1; apply H1; auto.
+  + simpl.
+    unfold canonical_model.
+    tauto.
+Qed.
+
+Theorem complete_intuitionistic_kripke: strongly_complete G SM (AllModel _).
+Proof.
+  assert (forall Phi x, ~ Phi |-- x -> ~ consequence (AllModel _) Phi x).
+  + intros.
+    assert (exists Psi: DCS, Included _ Phi (proj1_sig Psi) /\ ~ proj1_sig Psi |-- x).
+    Focus 1. {
+      apply Lindenbaum_lemma in H.
+      destruct H as [Psi [? [? ?]]].
+      exists (exist _ Psi H1).
+      simpl; auto.
+    } Unfocus.
+    destruct H0 as [Psi [? ?]].
+    intro.
+    specialize (H2 (canonical_model Psi)).
+    apply H1.
+    rewrite <- derivable_closed_element_derivable by (exact (proj1 (proj2_sig Psi))).
+    apply truth_lemma.
+    apply H2; intros; [hnf; auto |].
+    apply truth_lemma.
+    apply H0; auto.
+  + hnf; intros.
+    apply Classical_Prop.NNPP; intro; revert H0.
+    apply H; auto.
+Qed.
+
+End Completeness.
+
+
+Record canonical (Gamma: ProofTheory L) {MD: Model} {kMD: KripkeModel MD}  (M: Kmodel) {kiM: KripkeIntuitionisticModel (Kworlds M)} {SM: Semantics L MD} {kiSM: KripkeIntuitionisticSemantics L MD M SM}: Type := {
+  underlying_surj :> surjection (Kworlds M) (DCS Gamma);
+  canonical_relation_sound: forall m n m' n',
+    underlying_surj m m' ->
+    underlying_surj n n' ->
+    Korder m n ->
+    Included _ (proj1_sig n') (proj1_sig m');
+  canonical_relation_complete: forall n m' n',
+    underlying_surj n n' ->
+    Included _ (proj1_sig n') (proj1_sig m') ->
+    exists m,
+    underlying_surj m m' /\ Korder m n
+}.
+
+Lemma Lindenbaum_lemma {Gamma: ProofTheory L} {nGamma: NormalProofTheory L Gamma} {mpGamma: MinimunPropositionalLogic L Gamma} {ipGamma: IntuitionisticPropositionalLogic L Gamma}:
+  forall Phi x,
+    ~ Phi |-- x ->
+    exists Psi,
+      Included _ Phi Psi /\
+      ~ Psi |-- x /\
+      derivable_closed Psi /\
+      orp_witnessed Psi /\
+      consistent Psi.
+Proof.
+  intros.
+  assert (Countable expr) by (apply UnitarySeparationLanguage.formula_countable; auto).
+  set (step :=
+          fun n Phi x0 =>
+             Phi x0 \/
+            (X x0 n /\
+             ~ (Union _ Phi (Singleton _ x0)) |-- x)).
+  exists (LindenbaumConstruction step Phi).
+  assert (Included expr Phi (LindenbaumConstruction step Phi) /\
+          ~ LindenbaumConstruction step Phi |-- x /\
+          (~ LindenbaumConstruction step Phi |-- x ->
+           derivable_closed (LindenbaumConstruction step Phi)) /\
+          (~ LindenbaumConstruction step Phi |-- x ->
+           orp_witnessed (LindenbaumConstruction step Phi))).
+  Focus 2. {
+    destruct H0 as [? [? [? ?]]].
+    split; [| split; [| split; [| split]]]; auto.
+    rewrite consistent_spec.
+    intro; apply H1.
+    pose proof deduction_falsep_elim _ x H4.
+    auto.
+  } Unfocus.
+  split; [| split; [| split]].
+  + apply (Lindenbaum_spec_included _ _ 0).
+  + apply (Lindenbaum_spec_pos _ _
+            (fun xs => |-- multi_imp xs x)
+            (fun Phi => Phi |-- x)).
+    - intros; apply derivable_provable.
+    - intros ? ? ? ?; left; auto.
+    - apply H.
+    - intros.
+      destruct (Classical_Prop.classic (exists x0, X x0 n /\ ~ (Union _ S (Singleton _ x0)) |-- x)) as [[x0 [? ?]] |].
+      * intro; apply H2; clear H2.
+        eapply deduction_weaken; [| exact H3].
+        hnf; intros ? [? | [? ?]]; [left; auto |].
+        pose proof in_inj _ _ X _ _ _ H1 H2.
+        subst; right; constructor.
+      * intro; apply H0; clear H0.
+        eapply deduction_weaken; [| exact H2].
+        hnf; intros ? [? | [? ?]]; [auto |].
+        exfalso; apply H1; clear H1.
+        exists x0; auto.
+  + intros; hnf; intros.
+    destruct (im_inj _ _ X x0) as [n ?].
+    apply (Lindenbaum_spec_neg _ _ _ (S n)).
+    simpl.
+    unfold step at 1.
+    right; split; auto.
+    intro.
+    rewrite deduction_theorem in H3.
+    eapply deduction_weaken in H3; [| apply (Lindenbaum_spec_included _ _ n)].
+    pose proof deduction_modus_ponens _ _ _ H1 H3.
+    auto.
+  + intros; hnf; intros x0 y0 ?.
+    destruct (im_inj _ _ X x0) as [nx ?].
+    destruct (im_inj _ _ X y0) as [ny ?].
+    assert (LindenbaumChain step Phi (S nx) x0 \/ LindenbaumChain step Phi (S ny) y0) as HH;
+      [| destruct HH as [HH | HH]; apply Lindenbaum_spec_neg in HH; auto].
+    simpl.
+    unfold step at 1 3.
+    assert (~ Union _ (LindenbaumChain step Phi nx) (Singleton _ x0) |-- x \/
+            ~ Union _ (LindenbaumChain step Phi ny) (Singleton _ y0) |-- x) as HH;
+      [| destruct HH as [HH | HH]; auto].
+    apply Classical_Prop.not_and_or; intros [? ?].
+    rewrite deduction_theorem in H4, H5.
+    eapply deduction_weaken in H4; [| apply (Lindenbaum_spec_included _ _ nx)].
+    eapply deduction_weaken in H5; [| apply (Lindenbaum_spec_included _ _ ny)].
+    pose proof deduction_orp_elim (LindenbaumConstruction step Phi) x0 y0 x H4 H5.
+    apply (derivable_assum _ (x0 || y0)) in H1.
+    pose proof deduction_modus_ponens _ _ _ H1 H6.
+    auto.
+Qed.
+
+Lemma truth_lemma {Gamma: ProofTheory L} {nGamma: NormalProofTheory L Gamma} {mpGamma: MinimunPropositionalLogic L Gamma} {ipGamma: IntuitionisticPropositionalLogic L Gamma} {MD: Model} {kMD: KripkeModel MD} (M: Kmodel) {kiM: KripkeIntuitionisticModel (Kworlds M)} {SM: Semantics L MD} {kiSM: KripkeIntuitionisticSemantics L MD M SM}:
+  forall (X: canonical Gamma M),
+   (forall m Phi v,
+      X m Phi ->
+      (KRIPKE: M, m |= UnitarySeparationLanguage.varp v <-> proj1_sig Phi (UnitarySeparationLanguage.varp v))) ->
+   (forall m Phi,
+      X m Phi ->
+      forall x, KRIPKE: M, m |= x <-> proj1_sig Phi x).
+Proof.
+  intros.
+  rename H into ATOM_ASSUM, H0 into H.
+  pose proof (fun Phi: DCS Gamma => derivable_closed_element_derivable (proj1_sig Phi) (proj1 (proj2_sig Phi))).
+  revert Phi m H.
+  induction x; try solve [inversion H1]; intros.
+  + specialize (IHx1 Phi m H).
+    specialize (IHx2 Phi m H).
+    pose proof DCS_andp_iff (proj1_sig Phi) (proj1 (proj2_sig Phi)) x1 x2.
+    change (UnitarySeparationLanguage.andp x1 x2) with (x1 && x2).
+    rewrite sat_andp.
+    tauto.
+  + specialize (IHx1 Phi m H).
+    specialize (IHx2 Phi m H).
+    pose proof DCS_orp_iff (proj1_sig Phi) (proj1 (proj2_sig Phi)) (proj1 (proj2 (proj2_sig Phi))) x1 x2.
+    simpl in *.
+    change (UnitarySeparationLanguage.orp x1 x2) with (x1 || x2).
+    rewrite sat_orp.
+    tauto.
+  + split.
+    - intros.
+      rewrite H0.
+      change (UnitarySeparationLanguage.impp x1 x2) with (x1 --> x2) in *.
+      apply deduction_theorem.
+      apply Classical_Prop.NNPP; intro.
+      pose proof Lindenbaum_lemma _ _ H2.
+      destruct H3 as [Psi' [? [? ?]]].
+      set (Psi := exist _ Psi' H5: DCS Gamma).
+      change Psi' with (proj1_sig Psi) in H3, H4.
+      clearbody Psi; clear Psi' H5.
+      rewrite sat_impp in H1.
+      assert (Included _ (proj1_sig Phi) (proj1_sig Psi)) by (hnf; intros; apply H3; left; auto).
+      destruct (canonical_relation_complete _ _ X m Psi Phi H H5) as [n [? ?]].
+      specialize (H1 n H7).
+      rewrite IHx1, IHx2 in H1 by eauto.
+      assert (proj1_sig Psi x1) by (apply H3; right; constructor).
+      specialize (H1 H8).
+      specialize (H0 Psi x2).
+      rewrite H0 in H1; auto.
+    - intros.
+      change (UnitarySeparationLanguage.impp x1 x2) with (x1 --> x2) in *.
+      rewrite sat_impp; intros n ?H.
+      destruct (im_surj _ _ X n) as [Psi ?].
+      rewrite IHx1, IHx2 by eauto.
+      intros.
+      rewrite H0 in H1, H4 |- *.
+      eapply canonical_relation_sound in H2; [| eauto | eauto].
+      eapply deduction_weaken in H1; [| exact H2].
+      eapply deduction_modus_ponens; [exact H4 | exact H1].
+  + 
+  + pose proof sat_falsep m.
+    split; [intros; tauto | intros].
+    rewrite H0 in H2.
+    pose proof proj2_sig Phi.
+    destruct H3 as [_ [_ ?]].
+    rewrite consistent_spec in H3.
+    exfalso; apply H3; auto.
+  + auto.
+Qed.
+
+Definition canonical_frame {Gamma: ProofTheory L}: KripkeSemantics.frame.
+  refine (KripkeSemantics.Build_frame (DCS Gamma) (fun a b => Included _ (proj1_sig b) (proj1_sig a)) _).
+  constructor.
+  + hnf; intros.
+    hnf; intros; auto.
+  + hnf; intros.
+    hnf; intros; auto.
+Defined.
+
+Program Definition canonical_eval {Gamma: ProofTheory L}: Var -> KripkeSemantics.sem canonical_frame :=
+  fun p a => a (PropositionalLanguage.varp p).
+Next Obligation.
+  apply H; auto.
+Qed.
+
+Definition canonical_Kmodel {Gamma: ProofTheory L}: @Kmodel (KripkeSemantics.MD Var) (KripkeSemantics.kMD Var) :=
+  KripkeSemantics.Build_Kmodel Var canonical_frame canonical_eval.
+
+Definition canonical_model {Gamma: ProofTheory L} (Phi: DCS Gamma) : @model (KripkeSemantics.MD Var) :=
+  KripkeSemantics.Build_model Var canonical_Kmodel Phi.
+
+Definition canonical_Kmodel_surjection {Gamma: ProofTheory L}: surjection (@Kworlds (KripkeSemantics.MD Var) (KripkeSemantics.kMD Var) canonical_Kmodel) (DCS Gamma).
+Proof.
+  apply (FBuild_surjection _ _ id).
+  hnf; intros.
+  exists b; auto.
+Defined.
+
+Lemma canonical_model_canonical {Gamma: ProofTheory L}: @canonical Gamma (KripkeSemantics.MD Var) (KripkeSemantics.kMD Var) canonical_Kmodel (KripkeSemantics.kiM Var _) (KripkeSemantics.SM Var) (KripkeSemantics.kiSM Var _).
+Proof.
+  intros.
+  apply (Build_canonical _ _ _ _ _ _ _ canonical_Kmodel_surjection).
+  + intros.
+    change (DCS Gamma) in m, n.
+    change (m = m') in H.
+    change (n = n') in H0.
+    subst n' m'.
+    auto.
+  + intros.
+    change (DCS Gamma) in n, m'.
+    change (n = n') in H.
+    subst n.
+    exists m'.
+    split; auto.
+    change (m' = m').
+    auto.
+Defined.
 
 Lemma truth_lemma: forall (Phi: DCS Var G) x, canonical_model Var Phi |= x <-> proj1_sig Phi x.
 Proof.
